Fix wf

theories/tree_borrows/defs.v
@@ -40,9 +40,12 @@ Definition wf_scalar t sc := ∀ t' l, sc = ScPtr l (Tag t') → t' < t.
 
 (* mem ~ gmap loc scalar
 *)
-Definition same_blocks (hp:mem) (trs:trees) :=
-  dom trs ≡ set_map (fun l:loc => l.1) (dom hp).
 
+Definition blocks_in_heap (hp : mem) : gset positive := set_map fst (dom hp).
+Arguments blocks_in_heap / _.
+Definition same_blocks (hp:mem) (trs:trees) :=
+  dom trs = (set_map fst (dom hp) : gset _).
+Arguments same_blocks / _ _.
 (* OLD: forall blk l, is_Some (hp !! (blk, l)) -> is_Some (trs !! blk). *)
 (* FIXME: map fst (dom hp) === dom trs *)
 (* FIXME: forall blk, (exists l, is_Some (hp !! (blk, l))) <-> is_Some (trs !! blk). *)
